%%%%%%%%%%%%%%%%%%%%%%%%%%%%%%%%%%%%%%%%%%%%%%
%%                                          %%
%% USE THIS FILE TO SUBMIT YOUR SOLUTIONS   %%
%%                                          %%
%% You must have the usamts.tex file in     %%
%% the same directory as this file.         %%
%% You do NOT need to submit this file or   %%
%% usamts.tex with your solutions.  You     %%
%% only need to submit the output PDF file. %%
%%                                          %%
%% DO NOT ALTER THE FILE usamts.tex         %%
%%                                          %%
%% If you have any questions or problems    %%
%% using this file, or with LaTeX in        %%
%% general, please go to the LaTeX          %%
%% forum on the Art Of Problem Solving      %%
%% web site, and post your problem.         %%
%%                                          %%
%%%%%%%%%%%%%%%%%%%%%%%%%%%%%%%%%%%%%%%%%%%%%%

%%%%%%%%%%%%%%%%%%%%%%%%%%%%%%%%%%%%%%%%%%%%
%% DO NOT ALTER THE FOLLOWING LINES
\documentclass[12pt]{article}
\usepackage{amsmath,amssymb,amsthm,amsfonts,tabularx}
\usepackage[pdftex]{graphicx}
% \usepackage{mathptmx}
% \usepackage{geometry}
%  \geometry{
%  b5paper,
%  left=15mm,
%  right=15mm,
%  top=15mm,
%  bottom.
% }
\graphicspath{ {./images/} }
\usepackage{fancyhdr}
\pagestyle{fancy}
\usepackage{setspace}
\usepackage{csquotes}
\include{../formatting}

\renewcommand{\baselinestretch}{1}
%% DO NOT ALTER THE ABOVE LINES
%%%%%%%%%%%%%%%%%%%%%%%%%%%%%%%%%%%%%%%%%%%%


%% If you would like to use Asymptote within this document (which is optional), 
%% you can find out how at the following URL:
%%
%%   http://www.artofproblemsolving.com/Wiki/index.php/Asymptote:_Advanced_Configuration
%%
%% As explained there, you will want to uncomment the line below.  But be
%% sure to check the website because there are several other steps that must 
%% be followed.
%% \usepackage{asymptote}

\newtheorem*{prop}{Proposition}
\newtheorem*{corollary}{Corollary}
\newtheorem*{lemma}{Lemma}
\theoremstyle{remark}
\newtheorem*{defn}{Definition}

\newtheoremstyle{named}{}{}{}{}{\bfseries}{.}{.5em}{\thmnote{Problem #3}}
\theoremstyle{named}
\newtheorem*{theorem}{Theorem}

%% Enter your real name here
%% Example: \realname{David Patrick}
\realname{Hanting Zhang}
\pset{6}
\mathclass{425A}

\renewcommand{\bf}{\mathbf}
\renewcommand{\implies}{\Rightarrow}
\newcommand{\coimplies}{\Leftarrow}

\begin{document}

\begin{theorem}[5]
    For any two real sequences \(\{a_n\}, \{b_n\}\), prove that 
    \[\limsup_{n \to \infty} (a_n + b_n) \le \limsup_{n \to \infty} a_n + \limsup_{n \to \infty} b_n.\]
\end{theorem}

We first prove a useful lemma.

\begin{lemma}
    Let \(\{a_n\}\) be a sequence. Then \[\limsup_{n \to \infty} a_n = \lim_{n \to \infty} (\sup \{a_k \mid k \ge n\}).\]
\end{lemma}

\begin{proof}
    Define \(A_n = \sup \{a_k \mid k \ge n\}\) and \(\lim_{n \to \infty} A_n = L\). 
\end{proof}

\begin{proof}
    Let \(A_n = \sup \{a_k \mid k \ge n\}\) and \(B_n = \sup \{b_k \mid k \ge n\}\). Then for any \(k \ge n\), we have \(a_k + b_k \le A_n + B_n\), so the property of the supremum says that \(\sup \{a_k + b_k \mid k \ge n\} \le A_n + B_n\). This holds for all \(n \in \mathbb N\), so we take the limit to obtain
    \begin{align*}
        \limsup_{n \to \infty} (a_n + b_n) &= \lim_{n \to \infty} \sup \{a_k + b_k \mid k \ge n\} \\
        &\le \lim_{n \to \infty} A_n + \lim_{n \to \infty} B_n \\
        &= \limsup_{n \to \infty} a_n + \limsup_{n \to \infty} b_n,
    \end{align*}
    as desired.
\end{proof}

\begin{theorem}[7]
    Prove that the convergence of \(\sum a_n\) implies the convergence of 
    \[\sum \frac{\sqrt{a_n}}{n},\]
    if \(a_n \ge 0\).
\end{theorem}

\begin{proof}
    The idea to this proof is that we must somehow linearize \(\frac{\sqrt{a_n}}{n}\) by bounding it with \(p_n a_n + q_n\). Then all that is required for \[\sum \frac{\sqrt{a_n}}{n}\] to converge is for 
    \[\sum p_n a_n + q_n = \sum p_n a_n + \sum q_n\] to converge. 

    Indeed, pick \(p_n = 1\) and \(q_n = \frac{1}{n^2}\). Since \(a_n, n \ge 0\), we have 
    \begin{align*}
        0 &\le a_n^2 + \frac{a_n}{n^2} + \frac{1}{n^4} \\
        \implies \frac{a_n}{n^2} &\le a_n^2 + 2\frac{a_n}{n^2} + \frac{1}{n^4} = \left(a_n + \frac{1}{n^2}\right) \\
        \implies \frac{\sqrt{a_n}}{n} &\le a_n + \frac{1}{n^2}.
    \end{align*}
    Then both \(\sum p_n a_n = \sum a_n\) and \(\sum q_n = \sum n^{-2}\) clearly converge. Hence \(\sum \sqrt{a_n}/n\) converges.
\end{proof}

\begin{theorem}[8]
    If \(\sum a_n\) converges, and if \(\{b_n\}\) is monotonic and bounded, prove that \(\sum a_n b_n\) converges. 
\end{theorem}

\begin{proof}
    Since \(\{b_n\}\) is bounded and montonic, it converges to some \(b \in \mathbb R\). If \(b_n\) is increasing, set \(c_n = b - b_n\), otherwise \(c_n = b_n - b\). This new sequence \(c_n\) is decreasing and converges to \(0\) by construction, therefore we may apply Theorem 3.42 from the textbook to obtain the convergence of \(\sum a_n c_n\). 
    Whether we have \(c_n = b - b_n\) or \(c_n = b_n - b\), the sum \(\sum a_n c_n\) differs from \(\sum a_n b_n\) by some constant of \(\pm \sum a_n b\). Hence \(\sum a_n b_n\) converges.
\end{proof}

\end{document}